Regex/NFA/Compile.lean
@@ -7,65 +7,54 @@ open Regex.Data (Expr)
 
 namespace Regex.NFA
 
-def pushNode (nfa : NFA) (node : Node) (inBounds : node.inBounds (nfa.nodes.size + 1)) :
+def pushNode (nfa : NFA) (node : Node) :
   { nfa' : NFA // nfa.nodes.size < nfa'.nodes.size } :=
   let start := nfa.nodes.size
   let nodes := nfa.nodes.push node
-  have inBounds := by
-    intro i
-    simp [nodes]
-    rw [Array.get_push]
-    split
-    case isTrue h =>
-      have := nfa.inBounds ⟨i.val, h⟩
-      apply Node.inBounds_of_inBounds_of_le this (Nat.le_succ _)
-    case isFalse => exact inBounds
-  let nfa' : NFA := ⟨nodes, ⟨start, by simp [nodes]⟩, inBounds⟩
+  let nfa' : NFA := ⟨nodes, start⟩
 
   ⟨nfa', by simp [nodes]⟩
 
 @[simp]
-theorem pushNode_size {nfa : NFA} {node : Node} {inBounds : node.inBounds (nfa.nodes.size + 1)} :
-  (nfa.pushNode node inBounds).val.nodes.size = nfa.nodes.size + 1 := by
+theorem pushNode_size {nfa : NFA} {node : Node} :
+  (nfa.pushNode node).val.nodes.size = nfa.nodes.size + 1 := by
   simp [pushNode]
 
-theorem pushNode_get_lt {nfa : NFA} {node : Node} {inBounds : node.inBounds (nfa.nodes.size + 1)}
+theorem pushNode_get_lt {nfa : NFA} {node : Node}
   (i : Nat) (h : i < nfa.nodes.size) :
-  (nfa.pushNode node inBounds).val[i]'(Nat.lt_trans h (nfa.pushNode node inBounds).property) = nfa[i] := by
+  (nfa.pushNode node).val[i]'(Nat.lt_trans h (nfa.pushNode node).property) = nfa[i] := by
   simp [pushNode, get_eq_nodes_get]
   rw [Array.get_push_lt]
 
 @[simp]
-theorem pushNode_get_eq {nfa : NFA} {node : Node} {inBounds : node.inBounds (nfa.nodes.size + 1)} :
-  (nfa.pushNode node inBounds).val[nfa.nodes.size] = node := by
+theorem pushNode_get_eq {nfa : NFA} {node : Node} :
+  (nfa.pushNode node).val[nfa.nodes.size] = node := by
   simp [pushNode, get_eq_nodes_get]
 
-theorem pushNode_get {nfa : NFA} {node : Node} {inBounds : node.inBounds (nfa.nodes.size + 1)}
-  (i : Nat) (h : i < (nfa.pushNode node inBounds).val.nodes.size) :
-  (nfa.pushNode node inBounds).val[i]'h = if h' : i < nfa.nodes.size then nfa[i]'h' else node := by
+theorem pushNode_get {nfa : NFA} {node : Node}
+  (i : Nat) (h : i < (nfa.pushNode node).val.nodes.size) :
+  (nfa.pushNode node).val[i]'h = if h' : i < nfa.nodes.size then nfa[i]'h' else node := by
   simp at h
   cases Nat.lt_or_eq_of_le (Nat.le_of_succ_le_succ h) with
   | inl lt => simp [lt, pushNode_get_lt _ lt]
   | inr eq => simp [eq]
 
 @[simp]
-theorem pushNode_start_eq {nfa : NFA} {node : Node} {inBounds : node.inBounds (nfa.nodes.size + 1)} :
-  (nfa.pushNode node inBounds).val.start.val = nfa.nodes.size := rfl
+theorem pushNode_start_eq {nfa : NFA} {node : Node} : (nfa.pushNode node).val.start = nfa.nodes.size := rfl
 
 /--
   Compile a Regex and append the resulting nodes to the NFA. The nodes will transition to `next` on match.
 -/
-def pushRegex (nfa : NFA) (next : Fin nfa.nodes.size) :
-  Expr → { nfa' : NFA // nfa.nodes.size < nfa'.nodes.size }
-  | .empty => nfa.pushNode .fail (by simp)
-  | .epsilon => nfa.pushNode (.epsilon next) (by simp [Node.inBounds]; exact Nat.lt_trans next.isLt (Nat.lt_succ_self _))
-  | .char c => nfa.pushNode (.char c next) (by simp [Node.inBounds]; exact Nat.lt_trans next.isLt (Nat.lt_succ_self _))
-  | .classes cs => nfa.pushNode (.sparse cs next) (by simp [Node.inBounds]; exact Nat.lt_trans next.isLt (Nat.lt_succ_self _))
+def pushRegex (nfa : NFA) (next : Nat) : Expr → { nfa' : NFA // nfa.nodes.size < nfa'.nodes.size }
+  | .empty => nfa.pushNode .fail
+  | .epsilon => nfa.pushNode (.epsilon next)
+  | .char c => nfa.pushNode (.char c next)
+  | .classes cs => nfa.pushNode (.sparse cs next)
   | .group index r =>
     -- push the closing save node first
-    let nfa' := nfa.pushNode (.save (2 * index + 1) next) (by simp [Node.inBounds]; exact Nat.lt_trans next.isLt (Nat.lt_succ_self _))
+    let nfa' := nfa.pushNode (.save (2 * index + 1) next)
     let nfa'' := nfa'.val.pushRegex nfa'.val.start r
-    let nfa''' := nfa''.val.pushNode (.save (2 * index) nfa''.val.start) (by simp [Node.inBounds]; exact Nat.lt_trans nfa''.val.start.isLt (Nat.lt_succ_self _))
+    let nfa''' := nfa''.val.pushNode (.save (2 * index) nfa''.val.start)
 
     have property : nfa.nodes.size < nfa'''.val.nodes.size :=
       calc
@@ -78,20 +67,12 @@ def pushRegex (nfa : NFA) (next : Fin nfa.nodes.size) :
     -- TODO: it feels better to compile r₂ first to align with concat
     let nfa₁ := nfa.pushRegex next r₁
     let start₁ := nfa₁.val.start
-    let nfa₂ := nfa₁.val.pushRegex ⟨next, Nat.lt_trans next.isLt nfa₁.property⟩ r₂
+    let nfa₂ := nfa₁.val.pushRegex next r₂
     let start₂ := nfa₂.val.start
 
     let split := Node.split start₁ start₂
-    have inBounds : split.inBounds (nfa₂.val.nodes.size + 1) := by
-      have lt₁ : start₁ < nfa₂.val.nodes.size + 1 :=
-        calc
-          _ < _ := start₁.isLt
-          _ < _ := nfa₂.property
-          _ < _ := Nat.lt_succ_self _
-      have lt₂ : start₂ < nfa₂.val.nodes.size + 1 := Nat.lt_trans start₂.isLt (Nat.lt_succ_self _)
-      simp [split, lt₁, lt₂]
 
-    let nfa' := nfa₂.val.pushNode split inBounds
+    let nfa' := nfa₂.val.pushNode split
     have property : nfa.nodes.size < nfa'.val.nodes.size :=
       calc
         _ < _ := nfa₁.property
@@ -106,47 +87,22 @@ def pushRegex (nfa : NFA) (next : Fin nfa.nodes.size) :
     ⟨nfa₁, Nat.lt_trans nfa₂.property nfa₁.property⟩
   | .star r =>
     -- We need to generate a placeholder node first. We use `fail` for it because
-    -- 1. We'll use the fact that `fail` is a minimal element when strengthening induction hypotheis;
-    -- 2. We want to make sure `done` does not appear except at the first node.
-    -- 3. variants without data are represented as a boxed integer so there is one less allocation.
-    let placeholder := nfa.pushNode .fail (by simp)
-    let loopStart := placeholder.val.start
-    -- FIXME: generated code keeps `placeholder` alive, copying the array. Why?
-    let compiled := placeholder.val.pushRegex loopStart r
+    -- 1. We want to make sure `done` does not appear except at the first node.
+    -- 2. variants without data are represented as a boxed integer so there is one less allocation.
+    let placeholder := nfa.pushNode .fail
+    -- FIXME: generated code used to keep `placeholder` alive, copying the array. Investigate again
+    let compiled := placeholder.val.pushRegex nfa.nodes.size r
 
     -- Patch the placeholder node
-    have isLt : loopStart.val < compiled.val.nodes.size :=
+    have isLt : nfa.nodes.size < compiled.val.nodes.size :=
       calc
-        _ < _ := loopStart.isLt
+        _ < _ := placeholder.property
         _ < _ := compiled.property
-    let loopStart := ⟨loopStart.val, isLt⟩
 
     let split := Node.split compiled.val.start next
-    let patched := compiled.val.nodes.set loopStart split
-    have inBounds : ∀ i : Fin patched.size, patched[i].inBounds patched.size := by
-      simp [patched]
-      intro i
-      have hj : i < compiled.val.nodes.size := by
-        suffices i.val < (compiled.val.nodes.set loopStart split).size by
-          simp at this
-          exact this
-        exact i.isLt
-      rw [Array.get_set (hj := hj)]
-      split
-      case isTrue =>
-        have lt₁ : compiled.val.start < compiled.val.nodes.size := compiled.val.start.isLt
-        have lt₂ : next < compiled.val.nodes.size :=
-          calc
-            _ < _ := next.isLt
-            _ < _ := placeholder.property
-            _ < _ := compiled.property
-        simp [compiled, split, lt₁, lt₂]
-      case isFalse neq =>
-        have := compiled.val.inBounds ⟨i, hj⟩
-        simp at this
-        exact this
+    let patched := compiled.val.nodes.set ⟨nfa.nodes.size, isLt⟩ split
 
-    let nfa' := ⟨patched, loopStart.cast (by rw [Array.size_set]), inBounds⟩
+    let nfa' := ⟨patched, nfa.nodes.size⟩
     have property :=
       calc
         _ < _ := placeholder.property
@@ -155,48 +111,41 @@ def pushRegex (nfa : NFA) (next : Fin nfa.nodes.size) :
 
     ⟨nfa', property⟩
 
-def compile (r : Expr) : NFA := done.pushRegex ⟨0, by decide⟩ r
+def compile (r : Expr) : NFA := done.pushRegex 0 r
 
 -- Useful lemmas about the compilation
 def pushRegex.empty (eq : pushRegex nfa next .empty = result)
-  {motive : result = nfa.pushNode .fail (by simp) → P} : P := by
+  {motive : result = nfa.pushNode .fail → P} : P := by
   simp [pushRegex] at eq
   exact motive eq.symm
 
 def pushRegex.epsilon (eq : pushRegex nfa next .epsilon = result)
-  {motive : result = nfa.pushNode (.epsilon next) (by simp [Node.inBounds]; exact Nat.lt_trans next.isLt (Nat.lt_succ_self _)) → P} : P := by
+  {motive : result = nfa.pushNode (.epsilon next) → P} : P := by
   simp [pushRegex] at eq
   exact motive eq.symm
 
 def pushRegex.char (eq : pushRegex nfa next (.char c) = result)
-  {motive : result = nfa.pushNode (.char c next) (by simp [Node.inBounds]; exact Nat.lt_trans next.isLt (Nat.lt_succ_self _)) → P} : P := by
+  {motive : result = nfa.pushNode (.char c next) → P} : P := by
   simp [pushRegex] at eq
   exact motive eq.symm
 
 def pushRegex.sparse
   (eq : pushRegex nfa next (.classes c) = result)
-  {motive : result = nfa.pushNode (.sparse c next)
-  ((by simp [Node.inBounds]; exact Nat.lt_trans next.isLt (Nat.lt_succ_self _))) → P} : P := by
+  {motive : result = nfa.pushNode (.sparse c next) → P} : P := by
   simp [pushRegex] at eq
   exact motive eq.symm
 
 def pushRegex.group (eq : pushRegex nfa next (.group index r) = result)
-  {motive : ∀ nfa' nfa'' nfa''' property inBounds' inBounds''',
-    nfa' = nfa.pushNode (.save (2 * index + 1) next) inBounds' →
+  {motive : ∀ nfa' nfa'' nfa''' property,
+    nfa' = nfa.pushNode (.save (2 * index + 1) next) →
     nfa'' = nfa'.val.pushRegex nfa'.val.start r →
-    nfa''' = nfa''.val.pushNode (.save (2 * index) nfa''.val.start) inBounds''' →
+    nfa''' = nfa''.val.pushNode (.save (2 * index) nfa''.val.start) →
     result = ⟨nfa''', property⟩ →
     P
   } : P := by
-  have inBounds' : (Node.save (2 * index + 1) next).inBounds (Array.size nfa.nodes + 1) := by
-    simp [Node.inBounds]
-    exact Nat.lt_trans next.isLt (Nat.lt_succ_self _)
-  let nfa' := nfa.pushNode (.save (2 * index + 1) next) inBounds'
+  let nfa' := nfa.pushNode (.save (2 * index + 1) next)
   let nfa'' := nfa'.val.pushRegex nfa'.val.start r
-  have inBounds''' : (Node.save (2 * index) nfa''.val.start).inBounds (Array.size nfa''.val.nodes + 1) := by
-    simp [Node.inBounds]
-    exact Nat.lt_trans nfa''.val.start.isLt (Nat.lt_succ_self _)
-  let nfa''' := nfa''.val.pushNode (.save (2 * index) nfa''.val.start) inBounds'''
+  let nfa''' := nfa''.val.pushNode (.save (2 * index) nfa''.val.start)
 
   have property : nfa.nodes.size < nfa'''.val.nodes.size :=
     calc
@@ -204,41 +153,33 @@ def pushRegex.group (eq : pushRegex nfa next (.group index r) = result)
       _ < _ := nfa''.property
       _ < _ := nfa'''.property
 
-  exact motive nfa' nfa'' nfa''' property inBounds' inBounds''' rfl rfl rfl eq.symm
+  exact motive nfa' nfa'' nfa''' property rfl rfl rfl eq.symm
 
 def pushRegex.alternate (eq : pushRegex nfa next (.alternate r₁ r₂) = result)
-  {motive : ∀ nfa₁ start₁ nfa₂ start₂ inBounds nfa' property,
+  {motive : ∀ nfa₁ start₁ nfa₂ start₂ nfa' property,
     nfa₁ = nfa.pushRegex next r₁ →
     start₁ = nfa₁.val.start →
-    nfa₂ = nfa₁.val.pushRegex ⟨next, Nat.lt_trans next.isLt nfa₁.property⟩ r₂ →
+    nfa₂ = nfa₁.val.pushRegex next r₂ →
     start₂ = nfa₂.val.start →
-    nfa' = nfa₂.val.pushNode (.split start₁ start₂) inBounds →
+    nfa' = nfa₂.val.pushNode (.split start₁ start₂) →
     result = ⟨nfa', property⟩ →
     P
   } : P := by
   let nfa₁ := nfa.pushRegex next r₁
   let start₁ := nfa₁.val.start
-  let nfa₂ := nfa₁.val.pushRegex ⟨next, Nat.lt_trans next.isLt nfa₁.property⟩ r₂
+  let nfa₂ := nfa₁.val.pushRegex next r₂
   let start₂ := nfa₂.val.start
 
   let split := Node.split start₁ start₂
-  have inBounds : split.inBounds (nfa₂.val.nodes.size + 1) := by
-    have lt₁ : start₁ < nfa₂.val.nodes.size + 1 :=
-      calc
-        _ < _ := start₁.isLt
-        _ < _ := nfa₂.property
-        _ < _ := Nat.lt_succ_self _
-    have lt₂ : start₂ < nfa₂.val.nodes.size + 1 := Nat.lt_trans start₂.isLt (Nat.lt_succ_self _)
-    simp [split, lt₁, lt₂]
 
-  let nfa' := nfa₂.val.pushNode split inBounds
+  let nfa' := nfa₂.val.pushNode split
   have property : nfa.nodes.size < nfa'.val.nodes.size :=
     calc
       _ < _ := nfa₁.property
       _ < _ := nfa₂.property
       _ < _ := nfa'.property
 
-  exact motive nfa₁ start₁ nfa₂ start₂ inBounds nfa' property rfl rfl rfl rfl rfl eq.symm
+  exact motive nfa₁ start₁ nfa₂ start₂ nfa' property rfl rfl rfl rfl rfl eq.symm
 
 def pushRegex.concat (eq : pushRegex nfa next (.concat r₁ r₂) = result)
   {motive : ∀ nfa₂ nfa₁ property,
@@ -258,58 +199,31 @@ def pushRegex.concat (eq : pushRegex nfa next (.concat r₁ r₂) = result)
   exact motive nfa₂ nfa₁ property rfl rfl eq.symm
 
 def pushRegex.star (eq : pushRegex nfa next (.star r) = result)
-  {motive : ∀ placeholder compiled patched nfa' isLt inBounds property,
-    placeholder = nfa.pushNode .fail (by simp) →
-    compiled = placeholder.val.pushRegex ⟨nfa.nodes.size, placeholder.property⟩ r →
+  {motive : ∀ placeholder compiled patched nfa' property,
+    placeholder = nfa.pushNode .fail →
+    compiled = placeholder.val.pushRegex nfa.nodes.size r →
     patched = compiled.val.nodes.set
       ⟨nfa.nodes.size, Nat.lt_trans placeholder.property compiled.property⟩
       (Node.split compiled.val.start next) →
-    nfa' = ⟨patched, ⟨nfa.nodes.size, isLt⟩, inBounds⟩ →
+    nfa' = ⟨patched, nfa.nodes.size⟩ →
     result = ⟨nfa', property⟩ →
     P
   } : P := by
-  let placeholder := nfa.pushNode .fail (by simp)
-  let compiled := placeholder.val.pushRegex ⟨nfa.nodes.size, placeholder.property⟩ r
+  let placeholder := nfa.pushNode .fail
+  let compiled := placeholder.val.pushRegex nfa.nodes.size r
 
   -- Patch the placeholder node
   let loopStart : Fin _ := ⟨nfa.nodes.size, Nat.lt_trans placeholder.property compiled.property⟩
   let split := Node.split compiled.val.start next
   let patched := compiled.val.nodes.set loopStart split
-  have inBounds : ∀ i : Fin patched.size, patched[i].inBounds patched.size := by
-    simp [patched]
-    intro i
-    have hj : i < compiled.val.nodes.size := by
-      suffices i.val < (compiled.val.nodes.set loopStart split).size by
-        simp at this
-        exact this
-      exact i.isLt
-    rw [Array.get_set (hj := hj)]
-    split
-    case isTrue =>
-      have lt₁ : compiled.val.start < compiled.val.nodes.size := compiled.val.start.isLt
-      have lt₂ : next < compiled.val.nodes.size :=
-        calc
-          _ < _ := next.isLt
-          _ < _ := placeholder.property
-          _ < _ := compiled.property
-      simp [split, lt₁, lt₂]
-    case isFalse neq =>
-      have := compiled.val.inBounds ⟨i, hj⟩
-      simp at this
-      exact this
 
-  have isLt : nfa.nodes.size < patched.size :=
-    calc
-      _ < _ := placeholder.property
-      _ < _ := compiled.property
-      _ = _ := by simp [patched]
-  let nfa' : NFA := ⟨patched, ⟨nfa.nodes.size, isLt⟩, inBounds⟩
+  let nfa' : NFA := ⟨patched, nfa.nodes.size⟩
   have property :=
     calc
       _ < _ := placeholder.property
       _ < _ := compiled.property
       _ = nfa'.nodes.size := by simp [patched]
 
-  exact motive placeholder compiled patched nfa' isLt inBounds property rfl rfl rfl rfl eq.symm
+  exact motive placeholder compiled patched nfa' property rfl rfl rfl rfl eq.symm
 
 end NFA
