Regex/Regex/Basic.lean
@@ -4,6 +4,7 @@ import Regex.VM
 
 structure Regex where
   nfa : Regex.NFA
+  wf : nfa.WellFormed
   maxTag : Nat := nfa.maxTag
 deriving Repr
 
@@ -12,10 +13,10 @@ namespace Regex
 def parse (s : String) : Except String Regex := do
   let expr ← Regex.Syntax.Parser.parse s
   let nfa := Regex.NFA.compile expr
-  return { nfa := nfa }
+  return { nfa := nfa, wf := Regex.NFA.compile_wf }
 
 def parse! (s : String) : Regex :=
   let nfa := Regex.NFA.compile (Regex.Syntax.Parser.parse! s)
-  { nfa := nfa }
+  { nfa := nfa, wf := Regex.NFA.compile_wf }
 
 end Regex
