Regex/VM/Basic.lean
@@ -20,45 +20,45 @@ deriving Repr
 
 mutual
 
-def exploreεClosure (nfa : NFA) (pos : Pos)
+def exploreεClosure (nfa : NFA) (wf : nfa.WellFormed) (pos : Pos)
   (next : SparseSet nfa.nodes.size)
   (currentSave : Array (Option Pos)) (matched : Option (Array (Option Pos))) (saveSlots : Vec (Array (Option Pos)) nfa.nodes.size)
   (target : Fin nfa.nodes.size) (stack : Array (StackEntry nfa.nodes.size)) :
   (Option (Array (Option Pos)) × SparseSet nfa.nodes.size × Vec (Array (Option Pos)) nfa.nodes.size) :=
   if target ∈ next then
-    εClosure nfa pos next currentSave matched saveSlots stack
+    εClosure nfa wf pos next currentSave matched saveSlots stack
   else
     let next' := next.insert target
     match hn : nfa[target] with
     | .epsilon target' =>
-      have isLt := nfa.inBounds' target hn
-      exploreεClosure nfa pos next' currentSave matched saveSlots ⟨target', isLt⟩ stack
+      have isLt := wf.inBounds' target hn
+      exploreεClosure nfa wf pos next' currentSave matched saveSlots ⟨target', isLt⟩ stack
     | .split target₁ target₂ =>
       -- NOTE: unpacking the pair here confuses the simplifier
-      have isLt := nfa.inBounds' target hn
-      exploreεClosure nfa pos next' currentSave matched saveSlots ⟨target₁, isLt.1⟩ (stack.push (.explore ⟨target₂, isLt.2⟩))
+      have isLt := wf.inBounds' target hn
+      exploreεClosure nfa wf pos next' currentSave matched saveSlots ⟨target₁, isLt.1⟩ (stack.push (.explore ⟨target₂, isLt.2⟩))
     | .save offset target' =>
-      have isLt := nfa.inBounds' target hn
+      have isLt := wf.inBounds' target hn
       if h : offset < currentSave.size then
         let nextSave := currentSave.set ⟨offset, h⟩ pos
         let stack' := stack.push (.restore currentSave)
-        exploreεClosure nfa pos next' nextSave matched saveSlots ⟨target', isLt⟩ stack'
+        exploreεClosure nfa wf pos next' nextSave matched saveSlots ⟨target', isLt⟩ stack'
       else
-        exploreεClosure nfa pos next' currentSave matched saveSlots ⟨target', isLt⟩ stack
+        exploreεClosure nfa wf pos next' currentSave matched saveSlots ⟨target', isLt⟩ stack
     | .done =>
       let matched' := matched <|> currentSave
       let saveSlots' := saveSlots.set target target.isLt currentSave
-      εClosure nfa pos next' currentSave matched' saveSlots' stack
+      εClosure nfa wf pos next' currentSave matched' saveSlots' stack
     | .char _ _ =>
       let saveSlots' := saveSlots.set target target.isLt currentSave
-      εClosure nfa pos next' currentSave matched saveSlots' stack
+      εClosure nfa wf pos next' currentSave matched saveSlots' stack
     | .sparse _ _ =>
       let saveSlots' := saveSlots.set target target.isLt currentSave
-      εClosure nfa pos next' currentSave matched saveSlots' stack
-    | .fail => εClosure nfa pos next' currentSave matched saveSlots stack
+      εClosure nfa wf pos next' currentSave matched saveSlots' stack
+    | .fail => εClosure nfa wf pos next' currentSave matched saveSlots stack
 termination_by (next.measure, stack.size, 1)
 
-def εClosure (nfa : NFA) (pos : Pos)
+def εClosure (nfa : NFA) (wf : nfa.WellFormed) (pos : Pos)
   (next : SparseSet nfa.nodes.size)
   (currentSave : Array (Option Pos)) (matched : Option (Array (Option Pos))) (saveSlots : Vec (Array (Option Pos)) nfa.nodes.size)
   (stack : Array (StackEntry nfa.nodes.size)) :
@@ -70,13 +70,13 @@ def εClosure (nfa : NFA) (pos : Pos)
     let stack' := stack.pop
     have : stack'.size < stack.size := Array.lt_size_of_pop_of_not_empty _ hemp
     match entry with
-    | .explore target => exploreεClosure nfa pos next currentSave matched saveSlots target stack'
-    | .restore save => εClosure nfa pos next save matched saveSlots stack'
+    | .explore target => exploreεClosure nfa wf pos next currentSave matched saveSlots target stack'
+    | .restore save => εClosure nfa wf pos next save matched saveSlots stack'
 termination_by (next.measure, stack.size, 0)
 
 end
 
-def stepChar (nfa : NFA) (c : Char) (pos : Pos)
+def stepChar (nfa : NFA) (wf : nfa.WellFormed) (c : Char) (pos : Pos)
   (next : SparseSet nfa.nodes.size)
   (saveSlots : Vec (Array (Option Pos)) nfa.nodes.size)
   (target : Fin nfa.nodes.size) :
@@ -84,16 +84,16 @@ def stepChar (nfa : NFA) (c : Char) (pos : Pos)
   match hn : nfa[target] with
   | .char c' target' =>
     if c = c' then
-      have isLt := nfa.inBounds' target hn
+      have isLt := wf.inBounds' target hn
       let currentSave := saveSlots.get target target.isLt
-      exploreεClosure nfa pos next currentSave .none saveSlots ⟨target', isLt⟩ .empty
+      exploreεClosure nfa wf pos next currentSave .none saveSlots ⟨target', isLt⟩ .empty
     else
       (.none, next, saveSlots)
   | .sparse cs target' =>
     if c ∈ cs then
-      have isLt := nfa.inBounds' target hn
+      have isLt := wf.inBounds' target hn
       let currentSave := saveSlots.get target target.isLt
-      exploreεClosure nfa pos next currentSave .none saveSlots ⟨target', isLt⟩ .empty
+      exploreεClosure nfa wf pos next currentSave .none saveSlots ⟨target', isLt⟩ .empty
     else
       (.none, next, saveSlots)
   -- We don't need this as εClosure figures it out if there is a match
@@ -102,7 +102,7 @@ def stepChar (nfa : NFA) (c : Char) (pos : Pos)
   --   (.some saveSlots[target], next, saveSlots)
   | _ => (.none, next, saveSlots)
 
-def eachStepChar (nfa : NFA) (c : Char) (pos : Pos)
+def eachStepChar (nfa : NFA) (wf : nfa.WellFormed) (c : Char) (pos : Pos)
   (current : SparseSet nfa.nodes.size) (next : SparseSet nfa.nodes.size)
   (saveSlots : Vec (Array (Option Pos)) nfa.nodes.size) :
   (Option (Array (Option Pos)) × SparseSet nfa.nodes.size × Vec (Array (Option Pos)) nfa.nodes.size) :=
@@ -114,16 +114,16 @@ where
       (.none, next, saveSlots)
     else
       have hlt : i < current.count := Nat.lt_of_le_of_ne hle h
-      let result := stepChar nfa c pos next saveSlots current[i]
+      let result := stepChar nfa wf c pos next saveSlots current[i]
       match result.1 with
       | .none => go (i + 1) hlt result.2.1 result.2.2
       | .some _ => result
   termination_by current.count - i
 
-def captureNext (nfa : NFA) (it : String.Iterator) (saveSize : Nat) : Option (Array (Option Pos)) :=
+def captureNext (nfa : NFA) (wf : nfa.WellFormed) (it : String.Iterator) (saveSize : Nat) : Option (Array (Option Pos)) :=
   let saveSlots := Vec.ofFn (fun _ => initSave)
   let (matched, init, saveSlots) :=
-    exploreεClosure nfa it.pos .empty initSave .none saveSlots nfa.start #[]
+    exploreεClosure nfa wf it.pos .empty initSave .none saveSlots ⟨nfa.start, wf.start_lt⟩ #[]
   go it init .empty saveSlots matched
 where
   initSave : Array (Option Pos) := Array.ofFn (fun _ : Fin saveSize => none)
@@ -142,15 +142,15 @@ where
         let currentAndSaveSlots := if lastMatch.isNone then
           -- I think ignoring the match here is fine because the match must have happened at the initial exploration
           -- and `lastMatch` must have already captured that.
-          let explored := exploreεClosure nfa it.pos current initSave .none saveSlots nfa.start #[]
+          let explored := exploreεClosure nfa wf it.pos current initSave .none saveSlots ⟨nfa.start, wf.start_lt⟩ #[]
           explored.2
         else
           (current, saveSlots)
-        let stepped := eachStepChar nfa it.curr it.next.pos currentAndSaveSlots.1 next currentAndSaveSlots.2
+        let stepped := eachStepChar nfa wf it.curr it.next.pos currentAndSaveSlots.1 next currentAndSaveSlots.2
         go it.next stepped.2.1 current.clear stepped.2.2 (stepped.1 <|> lastMatch)
 
-def searchNext (nfa : NFA) (it : String.Iterator) : Option (Pos × Pos) := do
-  let slots ← captureNext nfa it 2
+def searchNext (nfa : NFA) (wf : nfa.WellFormed) (it : String.Iterator) : Option (Pos × Pos) := do
+  let slots ← captureNext nfa wf it 2
   let first ← (←slots.get? 0)
   let second ← (←slots.get? 1)
   pure (first, second)
